Small changes in declaration of cq-variables

src/main/isabelle/Test.thy
@@ -1,22 +1,8 @@
 theory Test
-  imports Main
+  imports QRHL
+  keywords "variables" :: thy_decl_block
+  and "variables2" :: thy_decl_block
 begin
-
-lemma x: fixes c :: int assumes "c = d" shows "True" ..
-
-context fixes a :: int begin
-
-ML {*
-val ctx = @{context}
-val T = TFree(("a"),@{sort type}) (* Note the incorrect "a" instead of "'a" *)
-val l = Free(("l"),T)
-val prop = HOLogic.mk_Trueprop (HOLogic.mk_eq (l,l)) (* prop = "l=l" *)
-fun tac {context=ctx, ...} = ALLGOALS (simp_tac ctx)
-val thm = Goal.prove ctx ["l"] [] prop tac (* proving prop *)
-val _ = @{thm x} OF [thm] (* Fails with "no unifiers". But succeeds if "fixes a" above is "fixes b" *)
-*}
-
-
 
 
 ML {*
@@ -33,51 +19,129 @@ in
 
 fun decl_var_hack name typ vartype = 
   Local_Theory.declaration {pervasive=true, syntax=false} (fn morph => Context.mapping (fn thy => thy)
-   (fn ctx => (@{print} morph; declare_variable ctx name (Morphism.typ morph typ) vartype)))
+   (fn ctx => (declare_variable ctx name (Morphism.typ morph typ) vartype)))
 
 end
 *}
 
-context
-  fixes a_var b_var c_var :: "int qvariable"
-  assumes "variable_name a_var = ''a''"
-  assumes "variable_name b_var = ''b''"
-  assumes "variable_name c_var = ''c''"
-  (* assumes [simp]: "distinct_qvars \<lbrakk>a,b,c\<rbrakk>" *)
-begin
+ML {*
+fun varname_assumption bind T = HOLogic.mk_eq 
+  (Const(@{const_name variable_name}, QRHL.mk_qvariableT T --> @{typ string}) $ 
+       Free(Binding.name_of bind ^ "_var", QRHL.mk_qvariableT T),
+   HOLogic.mk_string (Binding.name_of bind)) |> HOLogic.mk_Trueprop
+fun variables vars gthy = 
+let fun elems0 idx = [
+      Element.Fixes (map (fn (_,bind,T) => (Binding.suffix_name idx bind, SOME T, Mixfix.NoSyn)) vars),
+      Element.Fixes (map (fn (_,bind,T) => (Binding.suffix_name (idx^"_var") bind, SOME (QRHL.mk_qvariableT T), Mixfix.NoSyn)) vars),
+      Element.Assumes (map (fn (_,bind,T) => ((Binding.suffix_name (idx^"_varname") bind, @{attributes [simp]}),
+                             [(varname_assumption (Binding.suffix_name idx bind) T, [])])) vars)]
+    val elems = map elems0 ["", "1", "2"] |> List.concat
+    val (_,lthy) = Bundle.context [] elems gthy
+    val lthy2 = fold (fn (cq,bind,T) => fn lthy' => decl_var_hack (Binding.name_of bind) T cq lthy') vars lthy
+in lthy2 end
+*}
 
-local_setup {* decl_var_hack "a" @{typ int} QRHL.Classical *}
-local_setup {* decl_var_hack "b" @{typ int} QRHL.Classical *}
-local_setup {* decl_var_hack "c" @{typ int} QRHL.Classical *}
+ML {*
+fun variables_cmd vars gthy = 
+  let val ctxt = Context.proof_of gthy
+      val vars' = map (fn (a,b,c) => (a,b,Syntax.read_typ ctxt c)) vars
+  in
+    variables vars' gthy
+  end
+*}
+
+ML {*
+val parse_classical_quantum = (Parse.reserved "classical" >> K QRHL.Classical) || (Parse.reserved "quantum" >> K QRHL.Quantum)
+val _ =
+  Outer_Syntax.command @{command_keyword variables} "declare quantum/classical variables"
+    ((Parse.and_list (parse_classical_quantum -- Args.binding --| Parse.$$$ "::" -- Parse.typ >> (fn ((a,b),c) => (a,b,c))) >> 
+      (fn vars => Toplevel.open_target (variables_cmd vars)))
+        --| Parse.begin)
+*}
+
+(*ML {*
+  Outer_Syntax.command @{command_keyword variables2} "bla"
+  (Scan.succeed (Toplevel.open_target (fn gthy =>
+    let val lthy = Bundle.context [] [] gthy |> #2
+        val lthy2 = QRHL.declare_variable lthy @{binding "a"} @{typ bool} QRHL.Classical
+        val lthy3 = QRHL.declare_variable lthy2 @{binding "q"} @{typ nat} QRHL.Quantum
+  in lthy3 end
+  )))
+*}*)
+
+ML {*
+fun variables2 vars gthy =
+let val lthy = Bundle.context [] [] gthy |> #2
+    val lthy2 = fold (fn (cq,bind,T) => fn lthy' => QRHL.declare_variable lthy' bind T cq) vars lthy
+in lthy2 end
+*}
+
+ML {*
+fun variables2_cmd vars gthy = 
+  let val ctxt = Context.proof_of gthy
+      val vars' = map (fn (a,b,c) => (a,b,Syntax.read_typ ctxt c)) vars
+  in
+    variables2 vars' gthy
+  end
+*}
+
+ML {*
+val parse_classical_quantum = (Parse.reserved "classical" >> K QRHL.Classical) || (Parse.reserved "quantum" >> K QRHL.Quantum)
+val _ =
+  Outer_Syntax.command @{command_keyword variables2} "declare quantum/classical variables"
+    ((Parse.and_list (parse_classical_quantum -- Args.binding --| Parse.$$$ "::" -- Parse.typ >> (fn ((a,b),c) => (a,b,c))) >> 
+      (fn vars => Toplevel.open_target (variables2_cmd vars)))
+        --| Parse.begin)
+*}
+
+
+variables2 classical a :: int and quantum q :: nat begin
+term a_var
+term a
+term q
+thm a_varname
+
+lemma l: "variable_name a_var = ''a''" by simp
+
+end
+
+ML {*
+  Thm.cterm_of @{context} t1;
+  Thm.cterm_of @{context} t2
+*}
+
+lemma l: "variable_name a_var \<equiv> ''a''" sorry
+
+lemma "a_var=u" apply simp oops
+ML {* 
+@{thms a_varname}
+*}
+thm a_var
+ML Variable.declare_constraints
+
+variables
+  quantum a :: int and
+  classical b :: int and 
+  classical c :: int begin
+
+ML 1
 
 definition "p1 = [ assign a_var Expr[1], assign b_var Expr[2] ]"
 definition "p2 = [ assign a_var Expr[3], assign b_var Expr[4] ]"
 
+ML {* Tactics.take_n_thm @{context} 2 *}
 
-lemma take1: "s#l = [s]@l" by auto
-lemma take2: "s1#s2#l = [s1,s2]@l" by auto
+ML {* Type.constraint *}
 
-ML {* List.tabulate (3,fn i => i) *}
+lemma lem: "QRHL {Cla[True]} p1 p2 {Cla[True]}"
+  unfolding p1_def p2_def
+  using[[method_error=true]]
+  apply (seq 1 1 "Cla[a1=b1]")
+  sorry
 
-ML {* List.tabulate (3, fn i => Var(("s"^string_of_int (i+1),0),@{typ int})) *}
+end
 
-ML Array.tabulate
-
-ML {*
-*}
-
-ML {*
-take_n_thm @{context} 2 (* |> Thm.cterm_of @{context} *)
-*}
-
-ML {*
-val t = @{term "qrhl (expression qvariable_unit (\<lambda>x. \<CC>\<ll>\<aa>[True]))
-     [assign a_var (expression qvariable_unit (\<lambda>x. 1)), assign b_var (expression qvariable_unit (\<lambda>x. 2)) ]
-     [assign a_var (expression qvariable_unit (\<lambda>x. 3)), assign b_var (expression qvariable_unit (\<lambda>x. 4)) ]
-     (expression \<lbrakk>a1_var, a2_var, b1_var, b2_var\<rbrakk> (\<lambda>(a1, a2, b1, b2). \<CC>\<ll>\<aa>[a1 < a2] \<sqinter> \<CC>\<ll>\<aa>[b1 < b2]))"}
-*}
-
-
-
+variables classical a :: int and classical b :: int begin
+thm lem
 
 end
